{
 "cells": [
  {
   "cell_type": "markdown",
   "metadata": {},
   "source": [
    "If $x_1, ... x_n \\sim Unif(a, b)$ then the joint density can be written as:\n",
    "\n",
    "$$\n",
    "\\begin{align}\n",
    "p(x) & = \\prod_{i=1}^n (b - a)^{-1} \\textbf{1}_{\\{a \\le x_i \\le b\\}} \\\\\n",
    "& = (b - a)^{-n} \\textbf{1}_{\\{x_{(1)} \\ge a \\}} \\textbf{1}_{\\{x_{(n)} \\le b \\}}\n",
    "\\end{align}\n",
    "$$\n",
    "\n",
    "where $\\textbf{1}$ is the indicator function and $x_{(1)}$ is the min value and $x_{(n)}$ is the max value in the data."
   ]
  },
  {
   "cell_type": "markdown",
   "metadata": {},
   "source": [
    "(a) a = 0, b = $\\theta$\n",
    "\n",
    "The density is:\n",
    "\n",
    "$$p(x) = \\theta^{-n} \\textbf{1}_{\\{x_{(1)} \\ge 0 \\}} \\textbf{1}_{\\{x_{(n)} \\le \\theta \\}}$$\n",
    "\n",
    "and takes the form required by the factorization theorem with $h(x) = \\textbf{1}_{\\{0 \\le x_{(1)}\\}}$ and $g(t(x), \\theta) = \\theta^{-n} \\textbf{1}_{\\{x_{(n)} \\le \\theta \\}}$. So $t(x) = x_{(n)}$ is sufficient."
   ]
  },
  {
   "cell_type": "markdown",
   "metadata": {},
   "source": [
    "(b) a = $\\theta - 1$, b = $\\theta + 1$\n",
    "\n",
    "The density is:\n",
    "\n",
    "$$\n",
    "\\begin{align}\n",
    "p(x) & = 2^{-n} \\textbf{1}_{\\{x_{(1)} + 1 \\ge \\theta \\}} \\textbf{1}_{\\{x_{(n)} - 1 \\le \\theta  \\}} \\\\ \n",
    "& = 2^{-n} \\textbf{1}_{\\{-x_{(1)} - 1 \\le \\theta \\}} \\textbf{1}_{\\{x_{(n)} - 1 \\le \\theta  \\}}\n",
    "\\end{align}\n",
    "$$\n",
    "\n",
    "and takes the form required by the factorization theorem with $h(x) = 2^{-n}$ and $g(t(x), \\theta) = \\textbf{1}_{\\{x_{(1)} + 1 \\ge \\theta \\}} \\textbf{1}_{\\{x_{(n)} - 1 \\le \\theta  \\}}$. So $t(x) = max\\{-x_{(1)} - 1, x_{(n)} - 1 \\}$ is sufficient."
   ]
  },
  {
   "cell_type": "markdown",
   "metadata": {},
   "source": [
    "(c) The density is:\n",
    "\n",
    "$$p(x) = (\\theta_2 - \\theta_1)^{-n} \\textbf{1}_{\\{x_{(1)} \\ge \\theta_1 \\}} \\textbf{1}_{\\{x_{(n)} \\le \\theta_2 \\}} $$\n",
    "\n",
    "and takes the form required by the factorization theorem with $h(x) = 1$ and $g(t(x), \\theta) = p(x)$. So $t(x) = (x_{(1)}, x_{(n)} )$ is sufficient."
   ]
  },
  {
   "cell_type": "markdown",
   "metadata": {},
   "source": [
    "(d) a = $-\\theta$, b = $\\theta$\n",
    "\n",
    "The density is:\n",
    "\n",
    "$$\n",
    "\\begin{align}\n",
    "p(x) & = (2 \\theta)^{-n} \\textbf{1}_{\\{x_{(1)} \\ge -\\theta \\}} \\textbf{1}_{\\{x_{(n)} \\le \\theta \\}} \\\\\n",
    "& = (2 \\theta)^{-n} \\textbf{1}_{\\{-x_{(1)} \\le -\\theta \\}} \\textbf{1}_{\\{x_{(n)} \\le \\theta \\}}\n",
    "\\end{align}\n",
    "$$\n",
    "\n",
    "and takes the form required by the factorization theorem with $h(x) = (2 \\theta)^{-n}$ and $g(t(x), \\theta) = \\textbf{1}_{\\{x_{(1)} \\ge -\\theta \\}} \\textbf{1}_{\\{x_{(n)} \\le \\theta \\}}$. So $t(x) = max\\{-x_{(1)}, x_{(n)} \\}$ is sufficient."
   ]
  },
  {
   "cell_type": "markdown",
   "metadata": {},
   "source": [
    "(e) a = $\\theta$, b = 2$\\theta$\n",
    "The density is:\n",
    "\n",
    "$$p(x) = \\theta^{-n} \\textbf{1}_{\\{x_{(1)} \\ge \\theta \\}} \\textbf{1}_{\\{x_{(n)} / 2 \\le \\theta  \\}} = \\theta^{-n} \\textbf{1}_{\\{-x_{(1)} \\le \\theta \\}} \\textbf{1}_{\\{x_{(n)} / 2 \\le \\theta  \\}}$$\n",
    "\n",
    "and takes the form required by the factorization theorem with $h(x) = \\theta^{-n}$ and $g(t(x), \\theta) = \\textbf{1}_{\\{x_{(1)} \\ge \\theta \\}} \\textbf{1}_{\\{x_{(n)} / 2 \\le \\theta  \\}}$. So $t(x) = max\\{-x_{(1)}, x_{(n)/2} \\}$ is sufficient."
   ]
  },
  {
   "cell_type": "markdown",
   "metadata": {},
   "source": [
    "(f) If $(x_1, y_1), ... (x_n, y_n)$ are uniform in the circle with mean (0, 0) and radius $\\theta$ then the joint density and be written as:\n",
    "\n",
    "$$p(x, y) = \\prod_{i=1}^n (\\pi \\theta^2)^{-1} \\textbf{1}_{\\{x_{i}^2 + y_{i}^2 \\le \\theta^2 \\}} = \\pi^{-n} \\theta^{-2n} \\prod_{i=1}^n \\textbf{1}_{\\{x_{i}^2 + y_{i}^2 \\le \\theta^2 \\}} $$\n",
    "\n",
    "and takes the form required by the factorization theorem with $h(x, y) = \\pi^{-n}$ and $g(t(x, y), \\theta) = \\theta^{-2n} \\prod_{i=1}^n \\textbf{1}_{\\{x_{i}^2 + y_{i}^2 \\le \\theta^2 \\}}$. So $t(x) = (x_{1}^2 + y_{1}^2, ..., x_{n}^2 + y_{n}^2)$ is sufficient."
   ]
  },
  {
   "cell_type": "markdown",
   "metadata": {},
   "source": [
    "(g) If $(x_1, y_1), ... (x_n, y_n)$ are uniform in the square $(\\theta - 1, \\theta + 1) \\times (\\theta - 1, \\theta + 1)$ then the joint density and be written as:\n",
    "\n",
    "$$\n",
    "\\begin{align}\n",
    "p(x, y) & = \\prod_{i=1}^n [\\{(\\theta + 1) - (\\theta - 1)\\}^2]^{-1} \\textbf{1}_{ \\{ \\theta -1 \\le x_i \\le \\theta + 1, \\theta -1 \\le y_i \\le \\theta + 1 \\} } \\\\\n",
    "        & = 4^{-n}  \\prod_{i=1}^n \\textbf{1}_{ \\{ \\theta -1 \\le x_i \\le \\theta + 1 \\} } \\textbf{1}_{ \\{ \\theta -1 \\le y_i \\le \\theta + 1 \\} }\n",
    "\\end{align}\n",
    "$$\n",
    "\n",
    "and takes the form required by the factorization theorem with $h(x, y) = 4^{-n}$ and $g(t(x, y), \\theta) = \\prod_{i=1}^n \\textbf{1}_{ \\{ \\theta -1 \\le x_i \\le \\theta + 1 \\} } \\textbf{1}_{ \\{ \\theta -1 \\le y_i \\le \\theta + 1 \\} }$. Intuitively it makes sense that $t(x) = (x_1 y_1, ..., x_n y_n)$ is sufficient."
   ]
  },
  {
   "cell_type": "markdown",
   "metadata": {},
   "source": [
    "(h) If $x_1, ... x_n \\sim Exp(\\theta)$ then the joint density can be written as:\n",
    "\n",
    "$$\n",
    "\\begin{align}\n",
    "p(x) & = \\prod_{i=1}^n \\theta^{-1} \\exp [-x_i / \\theta]  \\\\\n",
    "& = \\theta^{-n} \\exp \\bigg[\\theta^{-1}  \\sum_{i=1}^n x_i \\bigg] \n",
    "\\end{align}\n",
    "$$\n",
    "\n",
    "and takes the form required by the factorization theorem with $h(x, y) = \\theta^{-n}$ and $g(t(x, y), \\theta) = \\exp \\bigg[\\theta^{-1}  \\sum_{i=1}^n x_i \\bigg]$. So $t(x) =  \\sum_{i=1}^n x_i$ is sufficient."
   ]
  },
  {
   "cell_type": "markdown",
   "metadata": {},
   "source": [
    "(i)  If $x_1, ... x_n \\sim Gamma(\\alpha, \\lambda)$ then the joint density can be written as:\n",
    "\n",
    "$$p(x) = \\prod_{i=1}^n \\frac{1}{\\Gamma(\\alpha)} \\lambda^ \\alpha x_i^{\\alpha - 1} \\exp(-\\lambda x_i)$$\n",
    "\n",
    "If $\\alpha$ is known then the density is given by:\n",
    "\n",
    "$$p(x) = \\Gamma(\\alpha)^{-n} \\lambda^{\\alpha n} \\prod_{i=1}^n x_i^{\\alpha - 1} \\exp \\bigg(-\\lambda \\sum_{i=1}^n x_i \\bigg)$$\n",
    "\n",
    "and takes the form required by the factorization theorem with $h(x) = \\Gamma(\\alpha)^{-n} \\lambda^{\\alpha n} \\prod_{i=1}^n x_i^{\\alpha - 1}$ and $g(t(x), \\lambda) = \\exp \\big(-\\lambda \\sum_{i=1}^n x_i \\big)$. So $t(x) =  \\sum_{i=1}^n x_i$ is sufficient.\n",
    "\n",
    "If $\\lambda$ is known then the density is given by:\n",
    "\n",
    "$$p(x) = \\exp \\bigg(-\\lambda \\sum_{i=1}^n x_i \\bigg) \\Gamma(\\alpha)^{-n} \\lambda^{\\alpha n} \\bigg( \\prod_{i=1}^n x_i \\bigg)^{\\alpha - 1}  $$\n",
    "\n",
    "and takes the form required by the factorization theorem with $h(x) = \\exp \\bigg(-\\lambda \\sum_{i=1}^n x_i \\bigg) \\Gamma(\\alpha)^{-n} \\lambda^{\\alpha n}$ and $g(t(x), \\alpha) = \\bigg( \\prod_{i=1}^n x_i \\bigg)^{\\alpha - 1}$. So $t(x) =  \\prod_{i=1}^n x_i$ is sufficient.\n",
    "\n",
    "If $(\\alpha, \\lambda)$ is unknown then the density is given by:\n",
    "\n",
    "$$p(x) = \\Gamma(\\alpha)^{-n} \\lambda^{\\alpha n} \\prod_{i=1}^n x_i^{\\alpha - 1} \\exp \\bigg(-\\lambda \\sum_{i=1}^n x_i \\bigg)$$\n",
    "\n",
    "and takes the form required by the factorization theorem with $h(x) = \\Gamma(\\alpha)^{-n} \\lambda^{\\alpha n}$ and $g(t(x), (\\alpha, \\lambda)) = \\prod_{i=1}^n x_i^{\\alpha - 1} \\exp \\bigg(-\\lambda \\sum_{i=1}^n x_i \\bigg)$. So $t(x) = \\bigg(\\prod_{i=1}^n x_i, \\sum_{i=1}^n x_i\\bigg)$ is sufficient."
   ]
  },
  {
   "cell_type": "markdown",
   "metadata": {},
   "source": [
    "(j) If $x_1, ... x_n \\sim Weibull(\\lambda, \\alpha)$ then the joint density can be written as:\n",
    "\n",
    "$$p(x) = \\prod_{i=1}^n \\alpha \\lambda (\\lambda x_i)^{\\alpha - 1} \\exp(-\\lambda x_i)^{\\alpha}$$\n",
    "\n",
    "If $(\\lambda, \\alpha)$ is unknown then the density is given by:\n",
    "\n",
    "$$p(x) = \\alpha^n \\lambda^{n + \\alpha - 1} \\bigg( \\prod_{i=1}^n x_i \\bigg)^{\\alpha - 1} \\exp \\bigg(-\\lambda \\sum_{i=1}^n x_i^{\\alpha} \\bigg)$$\n",
    "\n",
    "This does not take the form required by the factorization theorem due to the dependence on the parameter $\\alpha$ in the exponential term. As a result there is no non-trivial sufficient statistic in this case. Note that the data and the order statistics are always (trivial) sufficient statistics for any data set. A more [technical explanation](https://math.stackexchange.com/questions/636146/does-the-weibull-distribution-has-a-sufficient-statistic) in terms of a ratio of densities and permutations is given that I don't really understand yet.\n",
    "\n",
    "If $\\lambda$ is known then the same argument above holds.\n",
    "\n",
    "If $\\alpha$ is known then the density takes the form required by the factorization theorem with\n",
    "\n",
    "$h(x) = \\alpha^n \\lambda^{n + \\alpha - 1} \\bigg( \\prod_{i=1}^n x_i \\bigg)^{\\alpha - 1}$ and $g(t(x), \\lambda) = \\exp \\bigg(-\\lambda \\sum_{i=1}^n x_i^{\\alpha} \\bigg)$. So $t(x) = \\sum_{i=1}^n x_i^{\\alpha}$ is sufficient."
   ]
  },
  {
   "cell_type": "markdown",
   "metadata": {},
   "source": [
    "(k) If $x_1, ... x_n \\sim Beta(\\alpha, \\beta)$ then the joint density can be written as:\n",
    "\n",
    "$$\n",
    "\\begin{align}\n",
    "p(x) & = \\frac{\\Gamma (\\alpha, \\beta)^n} {\\Gamma (\\alpha)^n \\Gamma (\\beta)^n} \\prod_{i=1}^n  x_i^{\\alpha - 1} (1 - x_i)^{\\beta - 1} \\\\\n",
    "& = \\frac{\\Gamma (\\alpha, \\beta)^n} {\\Gamma (\\alpha)^n \\Gamma (\\beta)^n} \\bigg( \\prod_{i=1}^n  x_i \\bigg) ^{\\alpha - 1} \\bigg (\\prod_{i=1}^n (1 - x_i) \\bigg) ^{\\beta - 1}\n",
    "\\end{align}\n",
    "$$\n",
    "\n",
    "If $(\\alpha, \\beta)$ is unknown then the density is given by the above equation and takes the form required by the factorization theorem with $h(x) = \\frac{\\Gamma (\\alpha, \\beta)^n} {\\Gamma (\\alpha)^n \\Gamma (\\beta)^n}$ and $g(t(x), (\\alpha, \\beta)) = \\bigg( \\prod_{i=1}^n  x_i \\bigg) ^{\\alpha - 1} \\bigg (\\prod_{i=1}^n (1 - x_i) \\bigg) ^{\\beta - 1}$. So $t(x) = \\bigg(\\prod_{i=1}^n x_i, \\prod_{i=1}^n (1 - x_i) \\bigg)$ is sufficient.\n",
    "\n",
    "If $\\alpha$ is known then the density is given by the above equation and takes the form required by the factorization theorem with $h(x) = \\frac{\\Gamma (\\alpha, \\beta)^n} {\\Gamma (\\alpha)^n \\Gamma (\\beta)^n} \\bigg( \\prod_{i=1}^n  x_i \\bigg) ^{\\alpha - 1}$ and $g(t(x), \\beta) = \\bigg (\\prod_{i=1}^n (1 - x_i) \\bigg) ^{\\beta - 1}$. So $t(x) = \\prod_{i=1}^n (1 - x_i)$ is sufficient.\n",
    "\n",
    "If $\\beta$ is known then the density is given by the above equation and takes the form required by the factorization theorem with $h(x) = \\frac{\\Gamma (\\alpha, \\beta)^n} {\\Gamma (\\alpha)^n \\Gamma (\\beta)^n} \\bigg (\\prod_{i=1}^n (1 - x_i) \\bigg) ^{\\beta - 1}$ and $g(t(x), \\alpha) = \\bigg (\\prod_{i=1}^n x_i \\bigg) ^{\\alpha - 1}$. So $t(x) = \\prod_{i=1}^n x_i$ is sufficient."
   ]
  }
 ],
 "metadata": {
  "kernelspec": {
   "display_name": "Python 3",
   "language": "python",
   "name": "python3"
  },
  "language_info": {
   "codemirror_mode": {
    "name": "ipython",
    "version": 3
   },
   "file_extension": ".py",
   "mimetype": "text/x-python",
   "name": "python",
   "nbconvert_exporter": "python",
   "pygments_lexer": "ipython3",
   "version": "3.7.3"
  }
 },
 "nbformat": 4,
 "nbformat_minor": 4
}
